[/!\ Interface breaking change] Almost complete the implementation of the lexer, parser, and typer
Some macros are still missing. Extracting a standalone tool would help
writing more tests.

src/michocoq/micheline_parser.vy
@@ -7,10 +7,11 @@ Require Import micheline_syntax location.
 %token <location * location * Z> NUMBERt
 
 %start <loc_micheline> file
+%start <list (loc_micheline)> seq_file
 
-%type <location * location * list (loc_micheline) > args
+%type <location * location * list (loc_micheline) > atoms
 %type <list (loc_micheline) > seq
-%type <loc_micheline> arg atom app micheline
+%type <loc_micheline> atom app micheline
 
 %%
 
@@ -26,24 +27,32 @@ atom:
   | NUMBERt {
       let '((b, e), z) := $1 in
       Mk_loc_micheline (b, e, NUMBER z) }
+  | PRIMt {
+      let '((b, e), _) := $1 in
+      Mk_loc_micheline (b, e, PRIM $1 nil)
+    }
+  | LPAREN PRIMt RPAREN {
+      let '((b, e), _) := $2 in
+      Mk_loc_micheline (b, e, PRIM $2 nil)
+    }
+  | LPAREN app RPAREN { $2 }
   | LBRACE seq RBRACE {
       let '(b, _) := $1 in
       let '(_, e) := $3 in
       Mk_loc_micheline (b, e, SEQ $2) }
 ;
 
-arg:
-    atom { $1 }
-  | LPAREN app RPAREN { $2 }
-  | PRIMt {
-      let '((b, e), _) := $1 in
-      Mk_loc_micheline (b, e, PRIM $1 nil)
+app:
+    PRIMt atoms {
+      let '((b, _), _) := $1 in
+      let '((_, e), l) := $2 in
+      Mk_loc_micheline (b, e, PRIM $1 l)
     }
 ;
 
-args:
-    arg { let '(Mk_loc_micheline ((b, e), _)) := $1 in (b, e, cons $1 nil) }
-  | arg args {
+atoms:
+    atom { let '(Mk_loc_micheline ((b, e), _)) := $1 in (b, e, cons $1 nil) }
+  | atom atoms {
       let '(Mk_loc_micheline ((b, _), _)) := $1 in
       let '((_, e), l) := $2 in
       (b, e, cons $1 l)
@@ -52,25 +61,15 @@ args:
 
 micheline:
     atom { $1 }
-  | PRIMt {
-      let '((b, e), _) := $1 in
-      Mk_loc_micheline (b, e, PRIM $1 nil)
-    }
   | app { $1 }
 ;
 
 seq:
     { nil }
+  | micheline { cons $1 nil }
   | micheline SEMICOLON seq { cons $1 $3 }
 ;
 
-app:
-    PRIMt args {
-      let '((b, _), _) := $1 in
-      let '((_, e), l) := $2 in
-      Mk_loc_micheline (b, e, PRIM $1 l)
-    }
-;
-
 file: micheline EOF { $1 }
+seq_file: seq EOF { $1 }
 %%
