src/michocoq/main.v
@@ -2,11 +2,81 @@ Require Import String ZArith.
 Require micheline_lexer micheline_parser.
 Require untyped_syntax micheline2michelson typer.
 Require syntax.
+Require Import syntax_type.
 
-Module Main(ST : syntax.SelfType).
 
+Definition wrap_parser_result {A} r : error.M A :=
+  match r with
+  | micheline_parser.MenhirLibParser.Inter.Fail_pr =>
+    error.Failed _ error.Parsing
+  | micheline_parser.MenhirLibParser.Inter.Timeout_pr =>
+    error.Failed _ error.Parsing_Out_of_Fuel
+  | micheline_parser.MenhirLibParser.Inter.Parsed_pr m _ =>
+    error.Return _ m
+  end.
+
+Definition parse_micheline fuel (s : micheline_parser.MenhirLibParser.Inter.buffer)
+  : error.M micheline_syntax.loc_micheline :=
+  wrap_parser_result (micheline_parser.file fuel s).
+
+Definition lex_and_parse_micheline fuel input :
+  error.M (micheline_syntax.loc_micheline) :=
+  error.bind
+    (parse_micheline fuel)
+    (micheline_lexer.lex_micheline_to_parser input).
+
+Definition lex_and_parse_and_expand_type fuel input
+  : error.M type :=
+  error.bind
+    (fun m => micheline2michelson.micheline2michelson_type m)
+    (lex_and_parse_micheline fuel input).
+
+Definition get_file_object_from_string fuel input :=
+  error.bind
+    micheline2michelson.micheline2michelson_file
+    (error.bind
+       (fun x => wrap_parser_result (micheline_parser.seq_file fuel x))
+       (micheline_lexer.lex_micheline_to_parser input)).
+
+Definition get_parameter_type_from_string fuel input :=
+  error.bind
+    (fun a => error.Return _ a.(micheline2michelson.parameter))
+    (get_file_object_from_string fuel input).
+
+Definition get_storage_type_from_string fuel input :=
+  error.bind
+    (fun a => error.Return _ a.(micheline2michelson.storage))
+    (get_file_object_from_string fuel input).
+
+Module Type PARSEDSELFTYPE.
+  Parameter input : String.string.
+  Parameter fuel : Datatypes.nat.
+  Parameter success_param : error.Is_true (error.success (get_parameter_type_from_string fuel input)).
+  Parameter success_storage : error.Is_true (error.success (get_storage_type_from_string fuel input)).
+End PARSEDSELFTYPE.
+
+Module Type PARSEDFILE <: syntax.SelfType.
+  Parameter file_object : error.M micheline2michelson.untyped_michelson_file.
+  Parameter self_type : type.
+  Parameter storage_type : type.
+End PARSEDFILE.
+
+Module ParsedFile (ParsedSelfType : PARSEDSELFTYPE) <: PARSEDFILE.
+  Definition file_object := get_file_object_from_string ParsedSelfType.fuel ParsedSelfType.input.
+  Definition self_type :=
+    error.extract (error.bind (fun a => error.Return _ a.(micheline2michelson.parameter)) file_object)
+                  ParsedSelfType.success_param.
+  Definition storage_type :=
+    error.extract (error.bind (fun a => error.Return _ a.(micheline2michelson.storage)) file_object)
+                  ParsedSelfType.success_storage.
+End ParsedFile.
+
+Module Main(ST : PARSEDFILE).
+
+  (* Dummy context: getting the type of a contract always fails. *)
   Module ContractContext.
-    Definition get_contract_type (_ : syntax.contract_constant) := error.Failed syntax.type error.Typing.
+    Definition get_contract_type (_ : syntax.contract_constant) :
+      Datatypes.option type := None.
   End ContractContext.
 
   Module syntax := syntax.Syntax(ST)(ContractContext).
@@ -15,33 +85,147 @@ Module Main(ST : syntax.SelfType).
 
   Definition full_contract := syntax.full_contract.
 
-  Definition lex_and_parse_micheline (fuel : nat) (input : string) :
-    error.M (micheline_syntax.loc_micheline) :=
+  Definition code_M : error.M untyped_syntax.instruction :=
     error.bind
-      (fun s =>
-         match micheline_parser.file fuel s with
-         | micheline_parser.MenhirLibParser.Inter.Fail_pr =>
-           error.Failed _ error.Parsing
-         | micheline_parser.MenhirLibParser.Inter.Timeout_pr =>
-           error.Failed _ error.Parsing_Out_of_Fuel
-         | micheline_parser.MenhirLibParser.Inter.Parsed_pr m _ =>
-           error.Return _ m
-         end)
-      (micheline_lexer.lex_micheline_to_parser input).
+      (fun a => error.Return _ a.(micheline2michelson.code))
+      ST.file_object.
 
   Definition lex_and_parse_and_expand_and_type_full_contract
-             (fuel : nat) storage_ty (input : string)
-    : error.M (syntax.full_contract storage_ty) :=
-    error.bind
-      (fun i => typer.type_check_instruction_no_tail_fail typer.type_instruction i _ _)
-      (error.bind
-         (fun m => micheline2michelson.micheline2michelson_instruction m)
-         (lex_and_parse_micheline fuel input)).
+    : error.M (syntax.full_contract ST.storage_type) :=
+         error.bind
+           (fun i =>
+              typer.type_check_instruction_no_tail_fail typer.type_instruction i _ _)
+           code_M.
 
-  Definition lex_and_parse_and_expand_type (fuel : nat) (input : string)
-    : error.M syntax.type :=
-    error.bind
-      (fun m => micheline2michelson.micheline2michelson_type m)
-      (lex_and_parse_micheline fuel input).
+  Definition type_check : Datatypes.bool := error.success lex_and_parse_and_expand_and_type_full_contract.
 
 End Main.
+
+
+Module TestParsedSelfType <: PARSEDSELFTYPE.
+  Definition input : String.string :=
+    "parameter string;
+storage string;
+code {CAR; NIL operation; PAIR}".
+  Definition fuel := 60.
+  Definition success_param := I.
+  Definition success_storage := I.
+End TestParsedSelfType.
+
+Module TestSelfType := ParsedFile TestParsedSelfType.
+Eval compute in TestSelfType.file_object.
+Module TestMain := Main TestSelfType.
+Eval compute in TestMain.code_M.
+Eval compute in TestMain.lex_and_parse_and_expand_and_type_full_contract.
+Check (I : Bool.Is_true TestMain.type_check).
+
+
+
+Module MultisigParsedSelfType <: PARSEDSELFTYPE.
+  Definition input : String.string :=
+    "
+parameter (pair
+             (pair :payload
+                (nat %counter) # counter, used to prevent replay attacks
+                (or :action    # payload to sign, represents the requested action
+                   (pair :transfer    # transfer tokens
+                      (mutez %amount) # amount to transfer
+                      (contract %dest unit)) # destination to transfer to
+                   (or
+                      (option %delegate key_hash) # change the delegate to this address
+                      (pair %change_keys          # change the keys controlling the multisig
+                         (nat %threshold)         # new threshold
+                         (list %keys key)))))     # new list of keys
+             (list %sigs (option signature)));    # signatures
+
+storage (pair (nat %stored_counter) (pair (nat %threshold) (list %keys key))) ;
+
+code
+  {
+    UNPAIR ; SWAP ; DUP ; DIP { SWAP } ;
+    DIP
+      {
+        UNPAIR ;
+        # pair the payload with the current contract address, to ensure signatures
+        # can't be replayed accross different contracts if a key is reused.
+        DUP ; SELF ; ADDRESS ; PAIR ;
+        PACK ; # form the binary payload that we expect to be signed
+        DIP { UNPAIR @counter ; DIP { SWAP } } ; SWAP
+      } ;
+
+    # Check that the counters match
+    UNPAIR @stored_counter; DIP { SWAP };
+    ASSERT_CMPEQ ;
+
+    # Compute the number of valid signatures
+    DIP { SWAP } ; UNPAIR @threshold @keys;
+    DIP
+      {
+        # Running count of valid signatures
+        PUSH @valid nat 0; SWAP ;
+        ITER
+          {
+            DIP { SWAP } ; SWAP ;
+            IF_CONS
+              {
+                IF_SOME
+                  { SWAP ;
+                    DIP
+                      {
+                        SWAP ; DIIP { DIP { DUP } ; SWAP } ;
+                        # Checks signatures, fails if invalid
+                        CHECK_SIGNATURE ; ASSERT ;
+                        PUSH nat 1 ; ADD @valid } }
+                  { SWAP ; DROP }
+              }
+              {
+                # There were fewer signatures in the list
+                # than keys. Not all signatures must be present, but
+                # they should be marked as absent using the option type.
+                FAIL
+              } ;
+            SWAP
+          }
+      } ;
+    # Assert that the threshold is less than or equal to the
+    # number of valid signatures.
+    ASSERT_CMPLE ;
+    DROP ; DROP ;
+
+    # Increment counter and place in storage
+    DIP { UNPAIR ; PUSH nat 1 ; ADD @new_counter ; PAIR} ;
+
+    # We have now handled the signature verification part,
+    # produce the operation requested by the signers.
+    NIL operation ; SWAP ;
+    IF_LEFT
+      { # Transfer tokens
+        UNPAIR ; UNIT ; TRANSFER_TOKENS ; CONS }
+      { IF_LEFT {
+                  # Change delegate
+                  SET_DELEGATE ; CONS }
+                {
+                  # Change set of signatures
+                  DIP { SWAP ; CAR } ; SWAP ; PAIR ; SWAP }} ;
+    PAIR }".
+
+  Definition fuel := 600.
+
+  Definition lexed := Eval compute in error.extract (micheline_lexer.lex_micheline_to_parser input) I.
+  Definition parsed := Eval compute in error.extract (wrap_parser_result (micheline_parser.seq_file fuel lexed)) I.
+
+
+  Print parsed.
+  Definition file_object := Eval compute in get_file_object_from_string fuel input.
+  Print file_object.
+
+  Definition success_param := I.
+  Definition success_storage := I.
+End MultisigParsedSelfType.
+
+Module MultisigParsedFile := ParsedFile MultisigParsedSelfType.
+Module MultisigMain := Main MultisigParsedFile.
+
+Eval compute in MultisigMain.lex_and_parse_and_expand_and_type_full_contract.
+
+Check (I : Bool.Is_true MultisigMain.type_check).
