src/michocoq/syntax_type.v
@@ -1,0 +1,70 @@
+Inductive simple_comparable_type : Set :=
+| string
+| nat
+| int
+| bytes
+| bool
+| mutez
+| address
+| key_hash
+| timestamp.
+
+Inductive comparable_type : Set :=
+| Comparable_type_simple : simple_comparable_type -> comparable_type
+| Cpair : simple_comparable_type -> comparable_type -> comparable_type.
+
+Lemma comparable_type_dec (a b : comparable_type) : {a = b} + {a <> b}.
+Proof.
+  repeat decide equality.
+Defined.
+
+Inductive type : Set :=
+| Comparable_type : simple_comparable_type -> type
+| key : type
+| unit : type
+| signature : type
+| option : type -> type
+| list : type -> type
+| set : comparable_type -> type
+| contract : type -> type
+| operation : type
+| pair : type -> type -> type
+| or : type -> type -> type
+| lambda : type -> type -> type
+| map : comparable_type -> type -> type
+| big_map : comparable_type -> type -> type
+| chain_id : type.
+
+Fixpoint comparable_type_to_type (c : comparable_type) : type :=
+  match c with
+  | Comparable_type_simple a => Comparable_type a
+  | Cpair a b => pair (Comparable_type a) (comparable_type_to_type b)
+  end.
+
+
+Coercion comparable_type_to_type : comparable_type >-> type.
+Coercion Comparable_type_simple : simple_comparable_type >-> comparable_type.
+(* Coercion Comparable_type : simple_comparable_type >-> type. *)
+
+Fixpoint is_packable (a : type) : Datatypes.bool :=
+  match a with
+  | operation | big_map _ _ | contract _ => false
+  | Comparable_type _ | unit | signature | key | lambda _ _ | set _ | chain_id => true
+  | option ty
+  | list ty
+  | map _ ty => is_packable ty
+  | pair a b | or a b => is_packable a && is_packable b
+  end.
+
+Lemma type_dec (a b : type) : {a = b} + {a <> b}.
+Proof.
+  repeat decide equality.
+Defined.
+
+Lemma stype_dec (A B : Datatypes.list type) : {A = B} + {A <> B}.
+Proof.
+  decide equality; apply type_dec.
+Defined.
+
+Infix ":::" := (@cons type) (at level 60, right associativity).
+Infix "+++" := (@app type) (at level 60, right associativity).
